src/Init/Data/String/Pattern/Char.lean
@@ -8,6 +8,7 @@ module
 prelude
 public import Init.Data.String.Pattern.Basic
 public import Init.Data.Iterators.Consumers.Monadic.Loop
+import Init.Data.String.Basic
 import Init.Data.String.Termination
 
 set_option doc.verso true
